ballot sample now compiles (with small modifications)

Token.sol
@@ -1,0 +1,12 @@
+pragma solidity ^0.4.9;
+contract Token {
+  mapping (address => uint) balance;
+    function Token(uint n) {
+        balance[msg.sender] = n;
+    }
+    function send(address a, uint amount) {
+        if (balance[msg.sender] < amount) throw;
+        balance[msg.sender] -= amount;
+        balance[a] += amount;
+    } 
+}
