tofstar.js
@@ -19,7 +19,8 @@ var type_table = {
     uint: "UInt256.t",
     uint256: "UInt256.t",
     address: "UInt160.t",
-    bool: "bool"
+    bool: "bool",
+    bytes32: "UInt256.t"
 }
 
 function doConvert(part) {
@@ -33,6 +34,14 @@ convert.ElementaryTypeName = function (m) {
     return type_table[m.attributes.name]
 }
 
+convert.UserDefinedTypeName = function (m) {
+    return "struct_" + m.attributes.name
+}
+
+convert.ArrayTypeName = function (m) {
+    return "list (" + doConvert(m.children[0]) + ")"
+}
+
 convert.Mapping = function (m) {
     return doConvert(m.children[0]) + " -> " + doConvert(m.children[1])
 }
@@ -41,7 +50,7 @@ convert.IfStatement = function (a) {
     var str = ""
     str += "if " + doConvert(a.children[0]) + "\n"
     str += "then (" + doConvert(a.children[1]) + " ())\n"
-    str += "else " + (a.children[2] ? doConvert(a.children[2]) : "()") + ";\n"
+    str += "else (" + (a.children[2] ? doConvert(a.children[2]) + " ()" : "") + ");\n"
     return str
 }
 
@@ -58,8 +67,6 @@ convert.Return = function (a) {
 }
 
 convert.Literal = function (a) {
-    console.log("Literal " + a.attributes.type)
-    console.log(a)
     if (a.attributes.type2 == "address") {
         return "address_" + a.attributes.value
     }
@@ -72,13 +79,13 @@ convert.Literal = function (a) {
     if (a.attributes.type == "bool") {
         return a.attributes.value
     }
+    console.log("Literal " + a.attributes.type)
+    console.log(a)
 }
 
 var lits = {}
 
 function prepareLiteral(a) {
-    console.log("Literal " + a.attributes.type)
-    console.log(a)
     var name, type
     if (a.attributes.type2 == "address") {
         name = "address_" +  a.attributes.value
@@ -92,8 +99,12 @@ function prepareLiteral(a) {
         name = "uint256_" +  a.attributes.value
         type = "UInt256.uint_to_t"
     }
-    if (a.attributes.type == "bool") {
+    else if (a.attributes.type == "bool") {
         return ""
+    }
+    else {
+        console.log("Literal " + a.attributes.type)
+        console.log(a)
     }
     if (lits[name]) return ""
     lits[name] = true
@@ -104,7 +115,8 @@ convert.Throw = function () {
     return "raise SolidityThrow;"
 }
 
-//    convert.Identifier = a => a.attributes.value
+convert.PragmaDirective = function (a) {
+}
 
 convert.ForStatement = function (a) {
     var str = ""
@@ -117,17 +129,34 @@ convert.ForStatement = function (a) {
     return str
 }
 
+convert.WhileStatement = function (a) {
+    var str = ""
+    str += "let rec loop_"+a.id+" () : ML unit =\n"
+    str += "if not (" + doConvert(a.children[0]) + ") then () else (\n"
+    str += doConvert(a.children[1])
+    str += "loop_" + a.id + " ()) in loop_"+a.id+"();"
+    return str
+}
+
 convert.Identifier = a => {
-    console.log(a);
+    // console.log(a);
     if (a.attributes.scope == "local") return "!" + a.attributes.value
-    return a.attributes.value 
+    else if (a.attributes.scope == "param") return a.attributes.value
+    return "(!s)." + a.attributes.value 
 }
 
 convert.IndexAccess = function (a) {
-    return "get (!s)." + doConvert(a.children[0]) + " (" + doConvert(a.children[1]) + ")"
+    console.log(a)
+    if (a.children[0].attributes.type.match(/\[\] (storage ref|memory)/)) {
+        return "(list_nth (" + doConvert(a.children[0]) + ") (" + doConvert(a.children[1]) + "))"
+    }
+    return "(get " + doConvert(a.children[0]) + " (" + doConvert(a.children[1]) + "))"
 }
 
 convert.MemberAccess = function (a) {
+    if (a.attributes.member_name == "length") {
+        return "list_length " + "(" + doConvert(a.children[0]) + ")"
+    }
     return "(" + doConvert(a.children[0]) + ")." + a.attributes.member_name
 }
 
@@ -155,6 +184,7 @@ var op_table = {
     "bool ||": "bool_or",
     "uint256 !=": "op_disEquality",
     "address !=": "op_disEquality",
+    "address ==": "op_Equality",
 }
 
 function get_op(b) {
@@ -164,23 +194,54 @@ function get_op(b) {
     return op
 }
 
-convert.Assignment = function (a) {
-    var v = "???"
+function makeSetter(a, expr) {
 
-    if (a.children[0].name == "IndexAccess") {
-        if (a.attributes.operator == "=") v = doConvert(a.children[1])
-        else v = get_op(a) + " (" + doConvert(a.children[0]) + ") (" + doConvert(a.children[1]) + ")"
-        var b = a.children[0]
-        // return "set (" + doConvert(b.children[0]) + ") (" + doConvert(b.children[1]) + ") (" + v + ")"
-        return "s := {!s with " + doConvert(b.children[0]) + " = set (!s)." + doConvert(b.children[0]) + " (" + doConvert(b.children[1]) + ") (" + v + ") }"
+    if (a.name == "MemberAccess") {
+        var str = ""
+        var c = a
+        if (c.children[0].name == "IndexAccess") {
+            var b = c.children[0]
+            str += "let base = " + doConvert(b) + "in\n"
+            str += "let base = {base with " + a.attributes.member_name + " = (" + expr + ") } in\n"
+            str += makeSetter(b, "base")
+            return str
+        }
+        if (c.children[0].name == "Identifier" && c.children[0].attributes.scope == "local") {
+            var id = c.children[0].attributes.value
+            return id + " := { !" + id + " with " + a.attributes.member_name + " = " + expr + " }"
+        }
+    
     }
+
+    if (a.name == "IndexAccess") {
+        if (a.children[0].attributes.type.match(/\[\] (storage ref|memory)/)) {
+            return "s := {!s with " + a.children[0].attributes.value + " = list_set (" + doConvert(a.children[0]) + ") (" + doConvert(a.children[1]) + ") (" + expr + ") }"
+        }
+        return "s := {!s with " + a.children[0].attributes.value + " = set " + doConvert(a.children[0]) + " (" + doConvert(a.children[1]) + ") (" + expr + ") }"
+    }
+
+    if (a.name == "Identifier" && a.attributes.scope == "local") {
+        return a.attributes.value + " := " + expr
+    }
+    
+    if (a.name == "Identifier") {
+        return "s := {!s with " + a.attributes.value + " = (" + expr + ") }"
+    }
+    
+    console.log("setter")
+    console.log(a)
+}
+
+
+
+convert.Assignment = function (a) {
+    var v
 
     if (a.attributes.operator == "=") v = doConvert(a.children[1])
     else v = get_op(a) + " (" + doConvert(a.children[0]) + ") (" + doConvert(a.children[1]) + ")"
-    if (a.children[0].name == "Identifier" && a.children[0].attributes.scope == "local") {
-        return a.children[0].attributes.value + " := " + v
-    }
-    return doConvert(a.children[0]) + " := " + v
+    
+    return makeSetter(a.children[0], v)
+
 }
 
 convert.BinaryOperation = function (a) {
@@ -193,6 +254,70 @@ convert.UnaryOperation = function (a) {
 
 function convertType(v) {
     return doConvert(v.children[0])
+}
+
+function guessType(str) {
+    if (str.match(/int_const/)) return "uint256"
+    else return str
+}
+
+var conversion = {
+    "address uint256": "uint_to_address"
+}
+
+
+convert.FunctionCall = function (a) {
+    if (a.children[0].attributes.member_name == "transfer") {
+        return "()"
+    }
+    if (a.children[0].name == "ElementaryTypeNameExpression") {
+        var t = a.children[0].attributes.value + " " + guessType(a.children[1].attributes.type)
+        return conversion[t] + " " + doConvert(a.children[1])
+    }
+    if (a.children[0].name == "Identifier") {
+        console.log(a)
+        var str = ""
+        str += "let (ret,st) = method_" + a.children[0].attributes.value + " msg !s\n"
+        if (a.children.length == 1) str += "()"
+        else for (var i = 1; i < a.children.length; i++) {
+            str += doConvert(a.children[i])
+        }
+        str += " in\n (s := st; match ret with Some x -> x | None -> (* assert False ; *) raise SolidityBadReturn)"
+        return str
+    }
+    if (a.children[0].attributes.member_name == "push") {
+        // Expression representing array
+        var target = a.children[0].children[0]
+        var getter = doConvert(target)
+        return makeSetter(target, getter + " @ [ " + doConvert(a.children[1]) + "]")
+    }
+    console.log(a)
+}
+
+function flatten(lst) {
+    var res = []
+    lst.forEach(a => res = res.concat(a))
+    return res
+}
+
+function getChildren(a) {
+    if (!a.children) return []
+    return a.children.concat(flatten(a.children.map(b => getChildren(b))))
+}
+
+function checkTypes(a) {
+    var a1 = a.children[0]
+    var a2 = a.children[1]
+    if (a1.attributes.type.match(/int_const/)) {
+        a1.attributes.type2 = a2.attributes.type
+    }
+    if (a2.attributes.type.match(/int_const/)) {
+        a2.attributes.type2 = a1.attributes.type
+    }
+}
+
+convert.VariableDeclarationStatement = function (a) {
+    return "let " + a.children[0].attributes.name + " = alloc (" + doConvert(a.children[1]) + ") in\n"
 }
 
 function convertArgTypes(lst) {
@@ -210,48 +335,6 @@ function convertParams(lst) {
     return lst.children.map(a => a.attributes.name).join(" ")
 }
 
-convert.FunctionCall = function (a) {
-    if (a.children[0].attributes.member_name == "transfer") {
-        return "()"
-    }
-    if (a.children[0].name == "Identifier") {
-        var str = ""
-        str += "let (ret,st) = method_" + a.children[0].attributes.value + " msg !s\n"
-        for (var i = 1; i < a.children.length; i++) {
-            str += doConvert(a.children[i])
-        }
-        str += " in (s := st; match ret with Some x -> x | None -> (* assert False ; *) raise SolidityBadReturn)"
-        return str
-    }
-}
-
-function flatten(lst) {
-    var res = []
-    lst.forEach(a => res = res.concat(a))
-    return res
-}
-
-function getChildren(a) {
-    if (!a.children) return []
-    return a.children.concat(flatten(a.children.map(b => getChildren(b))))
-}
-
-function checkTypes(a) {
-    var a1 = a.children[0]
-    var a2 = a.children[1]
-    console.log(a)
-    if (a1.attributes.type.match(/int_const/)) {
-        a1.attributes.type2 = a2.attributes.type
-    }
-    if (a2.attributes.type.match(/int_const/)) {
-        a2.attributes.type2 = a1.attributes.type
-    }
-}
-
-convert.VariableDeclarationStatement = function (a) {
-    return "let " + a.children[0].attributes.name + " = alloc (" + doConvert(a.children[1]) + ") in\n"
-}
-
 convert.FunctionDefinition = function (a) {
     var str = ""
     // generate type
@@ -262,10 +345,10 @@ convert.FunctionDefinition = function (a) {
     str += "let ret = alloc None in\n"
     // Find all declared variables here, set them to local variable
     var table = {}
+    table["msg"] = "param"
     var children = getChildren(a.children[2])
-    console.log(children)
-    getChildren(a.children[2]).filter(a => a.name == "VariableDeclaration")
-                                         .forEach(a => { console.log(a); table[a.attributes.name] = "local"})
+    getChildren(a.children[2]).filter(a => a.name == "VariableDeclaration").forEach(a => table[a.attributes.name] = "local")
+    a.children[0].children.forEach(a => table[a.attributes.name] = "param")
     getChildren(a.children[2]).filter(a => a.name == "Identifier").forEach(a => a.attributes.scope = table[a.attributes.value])
     str += "try\n"
     str += doConvert(a.children[2]) + "\n"
@@ -278,14 +361,34 @@ function convertVar(v) {
     return v.attributes.name + " : " + doConvert(v.children[0]) + ";"
 }
 
+function makeStruct(a) {
+    var vars = a.children.filter(a => a.name == "VariableDeclaration")
+    return "noeq type struct_" + a.attributes.name + " = {\n" + vars.map(convertVar).join("\n") + "\n}\n"
+}
+
+function makeStructConstructor(a) {
+    var vars = a.children.filter(a => a.name == "VariableDeclaration")
+    var str = ""
+    str += "val method_" + a.attributes.name + " : msg -> state -> " + vars.map(a => convertType(a)).join(" -> ") + " -> ML (option (struct_" + a.attributes.name + ") * state)\n"
+    // generate body
+    str += "let method_" + a.attributes.name + " msg state " + vars.map(a => a.attributes.name).join(" ") + " = (Some ({\n"
+    vars.forEach(a => str += "  " + a.attributes.name + " = " + a.attributes.name + ";\n")
+    str += "}), state)\n"
+    return str
+}
+
 convert.ContractDefinition = function (c) {
+    // console.log(c)
     getChildren(c).filter(a => a.name == "BinaryOperation" || a.name == "Assignment").forEach(checkTypes)
     var str = ""
     str += "module " + c.attributes.name + "\n" + preamble
+    // structs
+    c.children.filter(a => a.name == "StructDefinition").forEach(a => str += makeStruct(a))
     // find variables
     var vars = c.children.filter(a => a.name == "VariableDeclaration")
     str += "\n\n\n(* Storage state *)\n"
     str += "noeq type state = {\n" + vars.map(convertVar).join("\n") + "\n}\n"
+    c.children.filter(a => a.name == "StructDefinition").forEach(a => str += makeStructConstructor(a))
     // literals
     getChildren(c).filter(a => a.name == "Literal").forEach(l => str += prepareLiteral(l) + "\n")
     // find methods
