Preamble.fst
@@ -2,6 +2,8 @@ open FStar.All
 open FStar.UInt160
 open FStar.UInt256
 open FStar.Heap
+open FStar.List
+open FStar.UInt
 
 type msg = {
   sender : UInt160.t;
@@ -13,6 +15,26 @@ let set #key #vl f ind x ind2 = if ind = ind2 then x else f ind2
 
 val get : #key:eqtype -> #vl:Type -> (key -> vl) -> key -> vl
 let get #key #vl f ind = f ind
+
+val address_to_uint : UInt160.t -> UInt256.t
+let address_to_uint a =
+  let x : uint_t 160 = UInt160.v a in
+  let y : uint_t 256 = UInt.to_uint_t 256 x in
+  UInt256.uint_to_t y
+
+val uint_to_address : UInt256.t -> UInt160.t
+let uint_to_address a = UInt160.uint_to_t (UInt.to_uint_t 160 (UInt256.v a))
+
+val list_length : #a:Type -> list a -> UInt256.t
+let list_length #a lst = UInt256.uint_to_t (UInt.to_uint_t 256 (List.length lst))
+
+val list_nth : #a:Type -> list a -> UInt256.t -> ML a
+let list_nth #a lst n = List.nth lst (UInt256.v n)
+
+val list_set : #a:Type -> list a -> UInt256.t -> a -> ML (list a)
+let list_set #a lst n elem =
+  let n = UInt256.v n in
+  List.mapi (fun i a -> if i = n then elem else a) lst 
 
 exception SolidityThrow
 exception SolidityReturn
@@ -28,13 +50,4 @@ let bool_and a b = a && b
 
 val bool_or : bool -> bool -> Tot bool
 let bool_or a b = a || b
-
-(*
-
-Could generate this kind of setters and getters in methods:
-
-let balance_set addr x = s := {!s with balance = set (!s).balance addr x } in
-let balance_get addr = get (!s).balance addr in
-
-*)
 
