Ballot.fst
@@ -1,0 +1,228 @@
+
+(******************)
+module Ballot
+open FStar.All
+open FStar.UInt160
+open FStar.UInt256
+open FStar.Heap
+open FStar.List
+open FStar.UInt
+
+type msg = {
+  sender : UInt160.t;
+  value: UInt256.t;
+}
+
+val set : #key:eqtype -> #vl:Type -> (key -> vl) -> key -> vl -> (key -> vl)
+let set #key #vl f ind x ind2 = if ind = ind2 then x else f ind2
+
+val get : #key:eqtype -> #vl:Type -> (key -> vl) -> key -> vl
+let get #key #vl f ind = f ind
+
+val address_to_uint : UInt160.t -> UInt256.t
+let address_to_uint a =
+  let x : uint_t 160 = UInt160.v a in
+  let y : uint_t 256 = UInt.to_uint_t 256 x in
+  UInt256.uint_to_t y
+
+val uint_to_address : UInt256.t -> UInt160.t
+let uint_to_address a = UInt160.uint_to_t (UInt.to_uint_t 160 (UInt256.v a))
+
+val list_length : #a:Type -> list a -> UInt256.t
+let list_length #a lst = UInt256.uint_to_t (UInt.to_uint_t 256 (List.length lst))
+
+val list_nth : #a:Type -> list a -> UInt256.t -> ML a
+let list_nth #a lst n = List.nth lst (UInt256.v n)
+
+val list_set : #a:Type -> list a -> UInt256.t -> a -> ML (list a)
+let list_set #a lst n elem =
+  let n = UInt256.v n in
+  List.mapi (fun i a -> if i = n then elem else a) lst 
+
+exception SolidityThrow
+exception SolidityReturn
+exception SolidityBadReturn
+
+val do_call : #state:Type -> #ret:Type -> (state -> ML (option ret * state)) -> state -> ML (option ret * state)
+let do_call #state #ret meth st =
+  try meth st
+  with SolidityThrow -> (None, st)
+
+val bool_and : bool -> bool -> Tot bool
+let bool_and a b = a && b
+
+val bool_or : bool -> bool -> Tot bool
+let bool_or a b = a || b
+
+noeq type struct_Voter = {
+weight : UInt256.t;
+voted : bool;
+delegate : UInt160.t;
+vote : UInt256.t;
+}
+noeq type struct_Proposal = {
+name : UInt256.t;
+voteCount : UInt256.t;
+}
+
+
+
+(* Storage state *)
+noeq type state = {
+chairperson : UInt160.t;
+voters : UInt160.t -> struct_Voter;
+proposals : list (struct_Proposal);
+}
+val method_Voter : msg -> state -> UInt256.t -> bool -> UInt160.t -> UInt256.t -> ML (option (struct_Voter) * state)
+let method_Voter msg state weight voted delegate vote = (Some ({
+  weight = weight;
+  voted = voted;
+  delegate = delegate;
+  vote = vote;
+}), state)
+val method_Proposal : msg -> state -> UInt256.t -> UInt256.t -> ML (option (struct_Proposal) * state)
+let method_Proposal msg state name voteCount = (Some ({
+  name = name;
+  voteCount = voteCount;
+}), state)
+let uint256_1 = UInt256.uint_to_t (1)
+let uint256_0 = UInt256.uint_to_t (0)
+
+
+
+
+
+
+
+
+
+
+
+
+
+(* Contract methods *)
+val method_Ballot : msg -> state -> list (UInt256.t) -> ML (option (unit) * state)
+let method_Ballot msg state proposalNames =
+let s = alloc state in
+let ret = alloc None in
+try
+s := {!s with chairperson = ((msg).sender) };
+let base = (get (!s).voters ((!s).chairperson))in
+let base = {base with weight = (uint256_1) } in
+s := {!s with voters = set (!s).voters ((!s).chairperson) (base) };
+let i = alloc (uint256_0) in
+let rec loop_66 () : ML unit =
+if not (UInt256.lt (!i) (list_length (proposalNames))) then () else (
+s := {!s with proposals = ((!s).proposals @ [ let (ret,st) = method_Proposal msg !s
+(list_nth (proposalNames) (!i))uint256_0 in
+ (s := st; match ret with Some x -> x | None -> (* assert False ; *) raise SolidityBadReturn)]) };i := UInt256.add_mod (!i) (uint256_1);loop_66 ()) in loop_66();
+(!ret, !s)
+with SolidityReturn -> (!ret, !s)
+
+
+val method_giveRightToVote : msg -> state -> UInt160.t -> ML (option (unit) * state)
+let method_giveRightToVote msg state voter =
+let s = alloc state in
+let ret = alloc None in
+try
+if bool_or (op_disEquality ((msg).sender) ((!s).chairperson)) (((get (!s).voters (voter))).voted)
+then (raise SolidityThrow; ())
+else ();
+
+let base = (get (!s).voters (voter))in
+let base = {base with weight = (uint256_1) } in
+s := {!s with voters = set (!s).voters (voter) (base) };
+(!ret, !s)
+with SolidityReturn -> (!ret, !s)
+
+
+val method_delegate : msg -> state -> UInt160.t -> ML (option (unit) * state)
+let method_delegate msg state to_ =
+let s = alloc state in
+let ret = alloc None in
+try
+let to = alloc (to_) in
+
+let sender = alloc ((get (!s).voters ((msg).sender))) in
+
+if (!sender).voted
+then (raise SolidityThrow; ())
+else ();
+
+if op_Equality (!to) ((msg).sender)
+then (raise SolidityThrow; ())
+else ();
+
+let rec loop_141 () : ML unit =
+if not (op_disEquality (((get (!s).voters (!to))).delegate) (uint_to_address uint256_0)) then () else (
+to := ((get (!s).voters (!to))).delegate;
+if op_Equality (!to) ((msg).sender)
+then (raise SolidityThrow; ())
+else ();
+loop_141 ()) in loop_141();
+sender := { !sender with voted = true };
+sender := { !sender with delegate = !to };
+let delegate = alloc ((get (!s).voters (!to))) in
+
+if (!delegate).voted
+then (let base = (list_nth ((!s).proposals) ((!delegate).vote))in
+let base = {base with voteCount = (UInt256.add_mod (((list_nth ((!s).proposals) ((!delegate).vote))).voteCount) ((!sender).weight)) } in
+s := {!s with proposals = list_set ((!s).proposals) ((!delegate).vote) (base) }; ())
+else (delegate := { !delegate with weight = UInt256.add_mod ((!delegate).weight) ((!sender).weight) }; ());
+
+(!ret, !s)
+with SolidityReturn -> (!ret, !s)
+
+
+val method_vote : msg -> state -> UInt256.t -> ML (option (unit) * state)
+let method_vote msg state proposal =
+let s = alloc state in
+let ret = alloc None in
+try
+let sender = alloc ((get (!s).voters ((msg).sender))) in
+
+if (!sender).voted
+then (raise SolidityThrow; ())
+else ();
+
+sender := { !sender with voted = true };
+sender := { !sender with vote = proposal };
+let base = (list_nth ((!s).proposals) (proposal))in
+let base = {base with voteCount = (UInt256.add_mod (((list_nth ((!s).proposals) (proposal))).voteCount) ((!sender).weight)) } in
+s := {!s with proposals = list_set ((!s).proposals) (proposal) (base) };
+(!ret, !s)
+with SolidityReturn -> (!ret, !s)
+
+
+val method_winningProposal : msg -> state -> unit -> ML (option (UInt256.t) * state)
+let method_winningProposal msg state () =
+let s = alloc state in
+let ret = alloc None in
+try
+let winningProposal = alloc (uint256_0) in
+
+let winningVoteCount = alloc (uint256_0) in
+
+let p = alloc (uint256_0) in
+let rec loop_264 () : ML unit =
+if not (UInt256.lt (!p) (list_length ((!s).proposals))) then () else (
+if UInt256.gt (((list_nth ((!s).proposals) (!p))).voteCount) (!winningVoteCount)
+then (winningVoteCount := ((list_nth ((!s).proposals) (!p))).voteCount;
+winningProposal := !p; ())
+else ();
+p := UInt256.add_mod (!p) (uint256_1);loop_264 ()) in loop_264();
+ret := Some(!winningProposal); raise SolidityReturn;
+(!ret, !s)
+with SolidityReturn -> (!ret, !s)
+
+
+val method_winnerName : msg -> state -> unit -> ML (option (UInt256.t) * state)
+let method_winnerName msg state () =
+let s = alloc state in
+let ret = alloc None in
+try
+ret := Some(((list_nth ((!s).proposals) (let (ret,st) = method_winningProposal msg !s
+() in
+ (s := st; match ret with Some x -> x | None -> (* assert False ; *) raise SolidityBadReturn)))).name); raise SolidityReturn;
+(!ret, !s)
+with SolidityReturn -> (!ret, !s)
